src/ext_traversal/ExtTraversal.v
@@ -8,15 +8,20 @@ Require Export ExtTravRelations.
 From imm Require Import TraversalProperties.
 Require Import ExtTraversalConfig.
 Require Import Lia.
+Require Import ImmFair.
+From imm Require Import FairExecution.
 
 Set Implicit Arguments.
 
 Section ExtTraversalConfig.
 Variable G : execution.
-Variable WF : Wf G.
-Variable COM : complete G.
-Variable sc : relation actid.
-Variable IMMCON : imm_consistent G sc.
+
+Hypothesis WF : Wf G.
+Hypothesis COM : complete G.
+Hypothesis sc : relation actid.
+Hypothesis IMMCON : imm_consistent G sc.
+Hypothesis FAIR: mem_fair G. 
+Hypothesis IMM_FAIR: imm_fair G sc. 
 
 (* Notation "'acts'" := (acts G). *)
 Notation "'sb'" := (sb G).
@@ -476,15 +481,15 @@ Qed.
 
 End Props.
 
-
 Lemma exists_ext_trav_step e (T: ext_trav_config)
       (N_FIN : next G (ecovered T) e)
       (ETCCOH : etc_coherent G sc T)
       (FINDOM: set_finite (acts_set G)):
   exists T', ext_trav_step T T'.
-Proof using WF IMMCON.
+Proof using WF IMMCON IMM_FAIR FAIR COM.
   edestruct exists_trav_step; eauto.
   { apply ETCCOH. }
+  { cdes FAIR. apply imm_s_rfppo.fsupp_ar_implies_fsupp_ar_rf_ppo_loc; auto. }    
   eapply trav_step_to_ext_trav_step; eauto.
 Qed.
 
